sym_eval works for trivialmem

src/CancelTacIL.v
@@ -1,6 +1,10 @@
+Require Import List Bool.
 Require MirrorShard.CancelTacBedrock.
 Require MirrorShard.ExprUnify.
-Require Import SepIL TacPackIL.
+Require Import MirrorShard.Expr.
+Require Import MirrorShard.Reflection.
+Require Import MirrorShard.Provers.
+Require Import ILEnv SepIL TacPackIL.
 
 Set Implicit Arguments.
 Set Strict Implicit.
@@ -10,3 +14,230 @@ Module CANCEL_TAC :=
                                     TacPackIL.SEP_LEMMA 
                                     ExprUnify.UNIFIER
                                     UNF.
+
+Section canceller.
+  Variable ts : list Expr.type.
+  Let types := Env.repr BedrockCoreEnv.core ts.
+
+
+
+(*
+  Theorem ApplyCancelSep_with_eq1 :
+    forall (funcs : functions types) (preds : SEP.predicates types)
+      (algos : TacPackIL.ILAlgoTypes.AllAlgos types)
+      (algosC : @TacPackIL.ILAlgoTypes.AllAlgos_correct types funcs preds algos)
+      (uvars : env types) (lhs rhs : SEP.sexpr types)
+      (hyps : exprs types)
+      (cr : CANCEL_LOOP.cancelResult types),
+      AllProvable funcs uvars nil hyps ->
+      (let bound := 10 in
+       let hints :=
+         match TacPackIL.ILAlgoTypes.Hints algos with
+           | None => {| UNF.Forward := nil ; UNF.Backward := nil |}
+           | Some x => x
+         end
+       in
+       let prover :=
+         match TacPackIL.ILAlgoTypes.Prover algos with
+           | None => Provers.trivialProver types
+           | Some x => x
+         end
+       in
+       let '(x,y) :=
+         CANCEL_LOOP.cancel (SEP.typeof_preds preds) prover (UNF.Forward hints) (UNF.Backward hints)
+         bound hyps (typeof_env uvars) nil lhs rhs in
+       (x, SEP.WellTyped_sexpr (typeof_funcs funcs) (SEP.typeof_preds preds) (typeof_env uvars) nil rhs && y) = (cr, true)) ->
+      CANCEL_LOOP.cancelResultD funcs preds uvars nil 0 cr ->
+      SEP.himp funcs preds uvars nil lhs rhs.
+  Proof.
+  Admitted.
+
+  Theorem ApplyCancelSep_with_eq2 :
+    forall (funcs : functions types) (preds : SEP.predicates types)
+      (algos : TacPackIL.ILAlgoTypes.AllAlgos types)
+      (algosC : @TacPackIL.ILAlgoTypes.AllAlgos_correct types funcs preds algos)
+      (uvars : env types) (lhs rhs : SEP.sexpr types)
+      (hyps : exprs types),
+      AllProvable funcs uvars nil hyps ->
+      (let bound := 10 in
+       let hints :=
+         match TacPackIL.ILAlgoTypes.Hints algos with
+           | None => {| UNF.Forward := nil ; UNF.Backward := nil |}
+           | Some x => x
+         end
+       in
+       let prover :=
+         match TacPackIL.ILAlgoTypes.Prover algos with
+           | None => Provers.trivialProver types
+           | Some x => x
+         end
+       in
+       let '(x,y) :=
+         CANCEL_LOOP.cancel (SEP.typeof_preds preds) prover (UNF.Forward hints) (UNF.Backward hints)
+         bound hyps (typeof_env uvars) nil lhs rhs in
+       if SEP.WellTyped_sexpr (typeof_funcs funcs) (SEP.typeof_preds preds) (typeof_env uvars) nil rhs && y then
+         CANCEL_LOOP.cancelResultD funcs preds uvars nil 0 x
+       else
+         SEP.himp funcs preds uvars nil lhs rhs) ->      
+      SEP.himp funcs preds uvars nil lhs rhs.
+  Proof.
+  Admitted.
+*)
+
+  Definition nsexprD (emp : hprop) (star : hprop -> hprop -> hprop) (ex : forall T : Type, (T -> hprop) -> hprop) (inj : Prop -> hprop) :=
+    fun (types : list Expr.type) (funcs : Expr.functions types)
+      (sfuncs : SEP.predicates types) =>
+      fix sexprD (meta_env var_env : Expr.env types) (s : SEP.sexpr types)
+      {struct s} : hprop :=
+      match s with
+        | SEP.Emp => emp
+        | SEP.Inj p =>
+          match Expr.exprD funcs meta_env var_env p Expr.tvProp with
+            | Some p0 => inj p0
+            | None => inj (SepExpr.BadInj p)
+          end
+        | SEP.Star l r =>
+          star (sexprD meta_env var_env l) (sexprD meta_env var_env r)
+        | SEP.Exists t b =>
+          ex _
+          (fun x : Expr.tvarD types t =>
+            sexprD meta_env (@existT _ (Expr.tvarD types) t x :: var_env) b)
+        | SEP.Func f b =>
+          match nth_error sfuncs f with
+            | Some f' =>
+              match
+                Expr.applyD (Expr.exprD funcs meta_env var_env) 
+                (SEP.SDomain f') b hprop (SEP.SDenotation f')
+                with
+                | Some p => p
+                | None => inj (SepExpr.BadPredApply f b var_env)
+              end
+            | None => inj (SepExpr.BadPred f)
+          end
+        | SEP.Const p => p
+      end.
+
+  Definition cancel (himp : hprop -> hprop -> Prop) (emp : hprop) (star : hprop -> hprop -> hprop) 
+    (ex : forall T : Type, (T -> hprop) -> hprop) (inj : Prop -> hprop)
+    (ts : list Expr.type)
+    (funcs : Expr.functions (Env.repr ILEnv.BedrockCoreEnv.core ts))
+    (preds : SEP.predicates (Env.repr ILEnv.BedrockCoreEnv.core ts))
+    (algos : TacPackIL.ILAlgoTypes.AllAlgos (Env.repr ILEnv.BedrockCoreEnv.core ts))
+    (uvars : Expr.env (Env.repr ILEnv.BedrockCoreEnv.core ts))
+    (lhs rhs : SEP.sexpr (Env.repr ILEnv.BedrockCoreEnv.core ts))
+    (hyps : Expr.exprs (Env.repr ILEnv.BedrockCoreEnv.core ts)) : Prop :=
+    let types := Env.repr ILEnv.BedrockCoreEnv.core ts in
+    let bound := 10 in
+    let hints :=
+      match TacPackIL.ILAlgoTypes.Hints algos with
+        | Some x => x
+        | None =>
+          {| TacPackIL.UNF.Forward := nil
+           ; TacPackIL.UNF.Backward := nil |}
+      end in
+    let prover :=
+      match TacPackIL.ILAlgoTypes.Prover algos with
+        | Some x => x
+        | None =>
+          Provers.trivialProver (Env.repr ILEnv.BedrockCoreEnv.core ts)
+      end in
+    let tfuncs := typeof_funcs funcs in
+    let tpreds := SEP.typeof_preds preds in
+    if SEP.WellTyped_sexpr tfuncs tpreds (typeof_env uvars) nil rhs then
+      match CANCEL_TAC.canceller tpreds (TacPackIL.UNF.Forward hints) (TacPackIL.UNF.Backward hints) prover (typeof_env uvars) hyps lhs rhs with
+        | None => 
+          himp (nsexprD emp star ex inj funcs preds uvars nil lhs)
+               (nsexprD emp star ex inj funcs preds uvars nil rhs)
+        | Some {| CANCEL_TAC.AllExt := new_vars
+                ; CANCEL_TAC.ExExt := new_uvars
+                ; CANCEL_TAC.Lhs := lhs'
+                ; CANCEL_TAC.Rhs := rhs'
+                ; CANCEL_TAC.Subst := subst |} =>
+          forallEach new_vars (fun nvs : env types =>
+             let var_env := nvs in
+             AllProvable_impl funcs uvars var_env
+               (CANCEL_TAC.existsSubst funcs var_env subst 0
+                 (map
+                   (fun x : sigT (tvarD types) =>
+                       existT (fun t : tvar => option (tvarD types t))
+                         (projT1 x) (Some (projT2 x))) uvars ++
+                    map
+                      (fun x : tvar =>
+                       existT (fun t : tvar => option (tvarD types t)) x None)
+                      new_uvars)
+                   (fun meta_env0 : env types =>
+                    AllProvable_and funcs meta_env0 var_env
+                      (himp
+                         (nsexprD emp star ex inj funcs preds meta_env0 var_env
+                            (SH.sheapD
+                               {|
+                               SH.impures := SH.impures lhs';
+                               SH.pures := nil;
+                               SH.other := SH.other lhs' |}))
+                         (nsexprD emp star ex inj funcs preds meta_env0 var_env
+                            (SH.sheapD
+                               {|
+                               SH.impures := SH.impures rhs';
+                               SH.pures := nil;
+                               SH.other := SH.other rhs' |})))
+                      (SH.pures rhs'))) (SH.pures lhs'))
+
+      end
+    else
+      himp (nsexprD emp star ex inj funcs preds uvars nil lhs)
+           (nsexprD emp star ex inj funcs preds uvars nil rhs).
+      
+
+  Theorem ApplyCancelSep_slice : forall (ts : list Expr.type)
+      (funcs : Expr.functions (Env.repr ILEnv.BedrockCoreEnv.core ts))
+      (preds : SEP.predicates (Env.repr ILEnv.BedrockCoreEnv.core ts))
+      (algos : TacPackIL.ILAlgoTypes.AllAlgos
+        (Env.repr ILEnv.BedrockCoreEnv.core ts)),
+      TacPackIL.ILAlgoTypes.AllAlgos_correct (types := Env.repr ILEnv.BedrockCoreEnv.core ts) funcs preds algos ->
+      forall (uvars : Expr.env (Env.repr ILEnv.BedrockCoreEnv.core ts))
+        (lhs rhs : SEP.sexpr (Env.repr ILEnv.BedrockCoreEnv.core ts))
+        (hyps : Expr.exprs (Env.repr ILEnv.BedrockCoreEnv.core ts)),
+        Expr.AllProvable funcs uvars nil hyps ->
+        (cancel himp emp star ex inj funcs preds algos uvars lhs rhs hyps) ->
+(*           
+         let '(x, y) :=
+           CancelTacIL.CANCEL_LOOP.cancel (SEP.typeof_preds preds)
+           prover (TacPackIL.UNF.Forward hints)
+           (TacPackIL.UNF.Backward hints) bound hyps
+           (Expr.typeof_env uvars) nil lhs rhs in
+           if (SEP.WellTyped_sexpr (Expr.typeof_funcs funcs)
+             (SEP.typeof_preds preds) (Expr.typeof_env uvars) nil rhs && y)%bool
+           then ncancelResultD himp emp star ex inj funcs preds uvars nil x
+           else himp (nsexprD emp star ex inj funcs preds uvars nil lhs)
+                     (nsexprD emp star ex inj funcs preds uvars nil rhs)) -> *)
+        SEP.himp funcs preds uvars nil lhs rhs.
+  Proof.
+    Opaque Env.repr.
+    intros. unfold cancel in *; simpl in *.    
+    consider (SEP.WellTyped_sexpr (typeof_funcs funcs) (SEP.typeof_preds preds) (typeof_env uvars) nil rhs); intros; eauto.
+    consider (CANCEL_TAC.canceller (SEP.typeof_preds preds)
+           (UNF.Forward
+              match ILAlgoTypes.Hints algos with
+              | Some x => x
+              | None => {| UNF.Forward := nil; UNF.Backward := nil |}
+              end)
+           (UNF.Backward
+              match ILAlgoTypes.Hints algos with
+              | Some x => x
+              | None => {| UNF.Forward := nil; UNF.Backward := nil |}
+              end)
+           match ILAlgoTypes.Prover algos with
+           | Some x => x
+           | None => trivialProver (Env.repr BedrockCoreEnv.core ts0)
+           end (typeof_env uvars) hyps lhs rhs); intros.
+    { eapply CANCEL_TAC.ApplyCancelSep_with_eq in H1; eauto. 
+      { destruct X. destruct (ILAlgoTypes.Hints algos); eauto using UNF.ForwardOk.
+        simpl. constructor. }
+      { destruct X. destruct (ILAlgoTypes.Hints algos); eauto using UNF.BackwardOk.
+        simpl. constructor. }
+      { destruct X. destruct (ILAlgoTypes.Prover algos); eauto using trivialProver_correct. }
+      { eapply typeof_funcs_WellTyped_funcs. } }
+    { apply H2. }
+  Qed.
+
+End canceller.
