src/ILTacLtac.v
@@ -103,7 +103,7 @@ Ltac sep_canceller isConst ext :=
                             Peano_dec.eq_nat_dec nat_rec nat_rect eq_rec_r eq_rect eq_rec 
                             f_equal eq_sym ]; exact proofs ) ; 
                       change (SEP.himp funcsV predsV uvars nil L R) ;
-                      apply (@ApplyCancelSep_slice typesV funcsV predsV 
+                      apply (@CancelTacIL.ApplyCancelSep_slice typesV funcsV predsV 
                         (TacPackIL.ILAlgoTypes.Algos ext typesV)
                         (@TacPackIL.ILAlgoTypes.Algos_correct ext typesV funcsV predsV)
                         uvars L R puresV puresPfV); 
@@ -129,6 +129,216 @@ Ltac sep_canceller isConst ext :=
  **     (this should be implmented using [cbv beta iota zeta delta [ ... ] in H])
  **     (it is recommended/necessary to call [sym_evaluator] or import its simplification)
  **)
+Ltac sym_eval isConst ext :=
+(*TIME  start_timer "sym_eval:init" ; *)
+  let rec init_from st :=
+    match goal with
+      | [ H : evalInstrs _ ?st' _ = Some st |- _ ] => init_from st'
+      | [ |- _ ] => st
+    end
+  in          
+  let stn_st_SF :=
+    match goal with
+      | [ H : PropX.interp _ (![ ?SF ] ?X) |- _ ] => 
+        let SF := eval unfold empB, injB, injBX, starB, exB, hvarB in SF in
+        constr:((X, (SF, H)))
+      | [ H : Structured.evalCond _ _ _ ?stn ?st = _ |- _ ] => 
+        let st := init_from st in
+        constr:(((stn, st), tt))
+      | [ H : IL.evalInstrs ?stn ?st _ = _ |- _ ] =>
+        let st := init_from st in
+        constr:(((stn, st), tt))
+      | [ |- _ ] => tt
+    end
+  in
+  let cs :=
+    match goal with
+      | [ H : PropX.codeSpec _ _ |- _ ] => H
+    end
+  in
+  let ext' := 
+    match ext with
+      | _ => eval cbv delta [ ext ] in ext
+      | _ => ext
+    end
+  in
+  match stn_st_SF with
+    | tt => idtac (* nothing to symbolically evluate *)
+    | ((?stn, ?st), ?SF) =>
+      match find_reg st Rp with
+        | (?rp_v, ?rp_pf) =>
+          match find_reg st Sp with
+            | (?sp_v, ?sp_pf) =>
+              match find_reg st Rv with
+                | (?rv_v, ?rv_pf) =>
+(*TIME                  stop_timer "sym_eval:init" ; *)
+(*TIME                  start_timer "sym_eval:gather_instrs" ; *)
+                  let all_instrs := get_instrs st in
+                  let all_props := 
+                    ReifyExpr.collect_props ltac:(ILTacCommon.reflectable shouldReflect)
+                  in
+                  let pures := ReifyExpr.props_types all_props in
+                  let regs := constr:((rp_v, (sp_v, (rv_v, tt)))) in
+(*TIME                  stop_timer "sym_eval:gather_instrs" ; *)
+                  (** collect the raw types **)
+(*TIME                  start_timer "sym_eval:reify" ; *)
+                  let Ts := constr:(Reify.Tnil) in
+                  let Ts k := 
+                    match SF with
+                      | tt => k Ts
+                      | (?SF,_) => (** TODO: a little sketchy since it is in CPS **)
+                        SEP_REIFY.collectTypes_sexpr ltac:(isConst) SF Ts k 
+                    end
+                  in
+                    Ts ltac:(fun Ts => 
+                  collectAllTypes_instrs all_instrs Ts ltac:(fun Ts => 
+                  ReifyExpr.collectTypes_exprs ltac:(isConst) regs Ts ltac:(fun Ts => 
+                  ReifyExpr.collectTypes_exprs ltac:(isConst) pures Ts ltac:(fun Ts => 
+                  (** check for potential universe problems **)
+                  match Ts with
+                    | context [ PropX.PropX ] => 
+                      fail 1000 "found PropX in types list"
+                        "(this causes universe inconsistencies)" Ts
+                    | context [ PropX.spec ] => 
+                      fail 1000 "found PropX.spec in types list"
+                        "(this causes universe inconsistencies)" Ts
+                    | _ => idtac
+                  end;
+                  (** elaborate the types **)
+                  let types_ := reduce_repr ext tt (TacPackIL.ILAlgoTypes.PACK.applyTypes (TacPackIL.ILAlgoTypes.Env ext) nil) in
+                  let types_ := ReifyExpr.extend_all_types Ts types_ in
+                  let typesV := fresh "types" in
+                  pose (typesV := types_);
+                  (** Check the types **)
+                  let pcT := constr:(Expr.tvType 0) in
+                  let stT := constr:(Expr.tvType 1) in
+                  (** build the variables **)
+                  let uvars := constr:(@nil (@sigT Expr.tvar (fun t : Expr.tvar => Expr.tvarD typesV t))) in
+                  let vars := uvars in
+                  (** build the base functions **)
+                  let funcs := reduce_repr ext tt (TacPackIL.ILAlgoTypes.PACK.applyFuncs (TacPackIL.ILAlgoTypes.Env ext) typesV (Env.repr (ILEnv.bedrock_funcs_r typesV) nil)) in
+                   (** build the base sfunctions **)
+(*                  let preds := constr:(@nil (@SEP.ssignature typesV pcT stT)) in *)
+                  let preds := reduce_repr ext tt (TacPackIL.ILAlgoTypes.PACK.applyPreds (TacPackIL.ILAlgoTypes.Env ext) typesV nil) in
+                  (** reflect the expressions **)
+                  ReifyExpr.reify_exprs ltac:(isConst) pures typesV funcs uvars vars ltac:(fun uvars funcs pures =>
+                  let proofs := ReifyExpr.props_proof all_props in
+                  
+                  ReifyExpr.reify_expr ltac:(isConst) rp_v typesV funcs uvars vars ltac:(fun uvars funcs rp_v  => 
+                  ReifyExpr.reify_expr ltac:(isConst) sp_v typesV funcs uvars vars ltac:(fun uvars funcs sp_v =>  
+
+                  ReifyExpr.reify_expr ltac:(isConst) rv_v typesV funcs uvars vars ltac:(fun uvars funcs rv_v => 
+                    let finish H  :=
+(*TIME                      start_timer "sym_eval:cleanup" ; *)
+                      ((try exact H) ||
+                       (let rec destruct_exs H :=
+                         match type of H with
+                           | Logic.ex _ =>
+                             destruct H as [ ? H ] ; destruct_exs H
+                           | forall x : ?T, _ =>
+                             let n := fresh in
+                             evar (n : T); 
+                             let e := eval cbv delta [ n ] in n in 
+                             specialize (H e)                             
+                           | (_ /\ (_ /\ _)) /\ (_ /\ _) =>
+                             destruct H as [ [ ? [ ? ? ] ] [ ? ? ] ];
+                               repeat match goal with
+                                        | [ H' : _ /\ _ |- _ ] => destruct H'
+                                      end
+                           | False => destruct H
+                           | ?G =>
+                             fail 100000 "bad result goal" G
+                         end
+                        in (* let fresh Hcopy := fresh "Hcopy" in
+                          let T := type of H in
+                            assert (Hcopy : T) by apply H; clear H; *) destruct_exs H))
+(*TIME                    ;  stop_timer "sym_eval:cleanup" *)
+                    in
+                    build_path typesV all_instrs st uvars vars funcs ltac:(fun uvars funcs is fin_state is_pf => 
+                      match SF with
+                        | tt => 
+(*TIME                          stop_timer "sym_eval:reify" ; *)
+                          (let funcsV := fresh "funcs" in
+                           pose (funcsV := funcs) ;
+                           let predsV := fresh "preds" in
+                           pose (predsV := preds) ;
+                           let uvarsV := fresh "uvars" in
+                           pose (uvarsV := uvars) ;
+                           let isV := fresh "path" in
+                           pose (isV := is) ;
+                           let isD := fresh "pathPf" in
+                           assert (isD : @SymIL.istreamD typesV (Env.repr (ILEnv.bedrock_funcs_r typesV) funcsV)
+                             uvarsV nil isV stn st fin_state) by (exact is_pf) ;
+                           let puresV := fresh "pures" in
+                           pose (puresV := pures) ;
+                           let puresPf := fresh "puresPf" in
+                           assert (puresPf : @Expr.AllProvable typesV (Env.repr (ILEnv.bedrock_funcs_r typesV) funcsV) uvars nil puresV) by (exact proofs) ;
+                           let new := fresh "after" in
+                           evar (new : Prop) ;
+                           let g := eval cbv delta [ new ] in new in
+                           let result := fresh in
+                           assert (result : g) by 
+                             (generalize (@SymILTac.ApplySymEval_slice_no_heap typesV funcsV predsV
+                                 (@TacPackIL.ILAlgoTypes.Algos ext typesV)
+                                 (@TacPackIL.ILAlgoTypes.Algos_correct ext typesV funcsV predsV)
+                                 stn uvarsV fin_state st isV isD cs sp_v rv_v rp_v puresV
+                                 sp_pf rv_pf rp_pf puresPf) ;
+                                let bl := constr:(Regs ::: ex ::: emp ::: star ::: inj ::: Evm_compute.Bnil) in
+                                let bl := add_bl ltac:(fun x => eval red in (Expr.Denotation x)) funcs bl in
+                                let bl := add_bl ltac:(fun x => eval red in (SEP.SDenotation x)) preds bl in
+                                subst funcsV predsV ; 
+                                evm computed_blacklist [ bl ] ;
+                                refine (fun x => x)) ;
+                             clear new puresPf puresV isD isV uvarsV predsV funcsV typesV ;
+                             clear_instrs all_instrs ;
+                             finish result) || fail 10000 "symbolic evaluation failed (no heap)"
+
+                        | (?SF, ?H_interp) =>
+                          SEP_REIFY.reify_sexpr ltac:(isConst) SF typesV funcs pcT stT preds uvars vars 
+                          ltac:(fun uvars funcs preds SF =>
+(*TIME                            stop_timer "sym_eval:reify" ; *)
+(*TIME                            start_timer "sym_eval:pose" ; *)
+                            (let funcsV := fresh "funcs" in
+                             pose (funcsV := funcs) ;
+                             let predsV := fresh "preds" in
+                             pose (predsV := preds) ;
+                             let uvarsV := fresh "uvars" in
+                             pose (uvarsV := uvars) ;
+                             let isV := fresh "path" in
+                             pose (isV := is) ;
+                             let isD := fresh "pathPf" in
+                             assert (isD : @SymIL.istreamD typesV (Env.repr (ILEnv.bedrock_funcs_r typesV) funcsV)
+                              uvarsV nil isV stn st fin_state) by (exact is_pf) ;
+                             let puresV := fresh "pures" in
+                             pose (puresV := pures) ;
+                             let puresPf := fresh "puresPf" in
+                             assert (puresPf : @Expr.AllProvable typesV (Env.repr (ILEnv.bedrock_funcs_r typesV) funcsV) uvars nil puresV) by (exact proofs) ;
+                             let new := fresh "after" in
+                             evar (new : Prop) ;
+                             let g := eval cbv delta [ new ] in new in
+                             let result := fresh in
+                             assert (result : g) by  
+                               (generalize (@SymILTac.ApplySymEval_slice_heap typesV funcsV predsV
+                                 (@TacPackIL.ILAlgoTypes.Algos ext typesV)
+                                 (@TacPackIL.ILAlgoTypes.Algos_correct ext typesV funcsV predsV)
+                                 stn uvarsV fin_state st isV isD cs sp_v rv_v rp_v puresV SF
+                                 sp_pf rv_pf rp_pf puresPf H_interp) ;
+                                let bl := constr:(Regs ::: PropX.interp ::: ex ::: emp ::: star ::: inj ::: Evm_compute.Bnil) in
+                                let bl := add_bl ltac:(fun x => eval red in (Expr.Denotation x)) funcs bl in
+                                let bl := add_bl ltac:(fun x => eval red in (SEP.SDenotation x)) preds bl in
+                                subst funcsV predsV ; 
+                                evm computed_blacklist [ bl ] ;
+                                refine (fun x => x)) ; 
+                             clear new H_interp puresPf puresV isD isV uvarsV predsV funcsV typesV ;
+                             clear_instrs all_instrs ;
+                             finish result) || fail 10000 "symbolic evaluation failed (with heap)" )
+                      end)))))  ))))
+              end
+          end
+      end
+  end.
+
+(*
 Ltac sym_eval isConst ext simplifier :=
 (*TIME  start_timer "sym_eval:init" ; *)
   let rec init_from st :=
@@ -262,7 +472,13 @@ Ltac sym_eval isConst ext simplifier :=
                           pose (funcsV := funcs) ;
                           let predsV := fresh "preds" in
                           pose (predsV := preds) ;
+                          let uvarsV := fresh "uvars" in
+                          pose (uvarsV := uvars) ;
 (*                          let ExtC := constr:(@Algos_correct _ _ _ _ _ _ ext typesV funcsV predsV) in *)
+                          generalize (@SymILTac.ApplySymEval_slice_no_heap typesV funcsV predsV
+                            (@ILAlgoTypes.Algos ext typesV) (@ILAlgoTypes.Algos_correct ext typesV funcsV predsV)
+                            stn uvarsV)
+(*
                           generalize (@SymILTac.stateD_proof_no_heap typesV funcsV predsV
                             uvars st sp_v rv_v rp_v 
                             sp_pf rv_pf rp_pf pures proofs cs stn) ;
@@ -274,7 +490,8 @@ Ltac sym_eval isConst ext simplifier :=
                           || fail 100000 "couldn't apply sym_eval_any! (non-SF case)"); 
                           first [ simplifier typesV funcsV predsV H_stateD | fail 100000 "simplifier failed! (non-SF)" ] ;
                           try clear typesV funcsV predsV ;
-                          first [ finish H_stateD (*; clear_instrs all_instrs*) | fail 100000 "finisher failed! (non-SF)" ]
+                          first [ finish H_stateD (*; clear_instrs all_instrs*) | fail 100000 "finisher failed! (non-SF)" ] 
+*)
                         | (?SF, ?H_interp) =>
                           SEP_REIFY.reify_sexpr ltac:(isConst) SF typesV funcs pcT stT preds uvars vars 
                           ltac:(fun uvars funcs preds SF =>
@@ -284,6 +501,10 @@ Ltac sym_eval isConst ext simplifier :=
                             pose (funcsV := funcs) ;
                             let predsV := fresh "preds" in
                             pose (predsV := preds) ;
+                            let uvarsV := fresh "uvars" in
+                            pose (uvarsV := uvars) ;
+                              idtac
+(*
 (*                            let ExtC := constr:(@Algos_correct ext typesV funcsV predsV) in *)
 (*TIME                            stop_timer "sym_eval:pose" ; *)
 (*TIME                            start_timer "sym_eval:apply_stateD_proof" ; *)
@@ -319,9 +540,11 @@ Ltac sym_eval isConst ext simplifier :=
 (*TIME                             start_timer "sym_eval:clear" ; *)
                             try clear typesV funcsV predsV ;
 (*TIME                             stop_timer "sym_eval:clear" ; *)
-                            first [ finish H_interp ; clear_instrs all_instrs | fail 100000 "finisher failed! (SF)" ])
+                            first [ finish H_interp ; clear_instrs all_instrs | fail 100000 "finisher failed! (SF)" ]
+*) )
                       end)))))  ))))
               end
           end
       end
   end.
+*)
